More work

src/Denote.v
@@ -14,6 +14,7 @@ Require Import Category.Theory.Functor.
 
 Require Import Solver.Lib.
 Require Import Solver.Expr.
+Require Import Solver.Normal.
 
 Generalizable All Variables.
 
@@ -26,7 +27,7 @@ Context {C : Category}.
 Variable objs : obj_idx -> C.
 Variable arrs : ∀ f : arr_idx, option (∃ x y, objs x ~{C}~> objs y).
 
-Fixpoint term_denote dom cod (e : Term) : option (objs dom ~{C}~> objs cod) :=
+Fixpoint termD dom cod (e : Term) : option (objs dom ~{C}~> objs cod) :=
   match e with
   | Identity _ =>
       match Eq_eq_dec cod dom with
@@ -47,22 +48,213 @@ Fixpoint term_denote dom cod (e : Term) : option (objs dom ~{C}~> objs cod) :=
     | _ => None
     end
   | Compose mid f g =>
-    match term_denote mid cod f, term_denote dom mid g with
+    match termD mid cod f, termD dom mid g with
     | Some f, Some g => Some (f ∘ g)
     | _, _ => None
     end
   end.
 
-Fixpoint expr_denote (e : Expr) : Type :=
+Fixpoint arrowsD dom cod `(fs : list (Arrow t)) :
+  option (objs dom ~{C}~> objs cod) :=
+  match fs with
+  | nil =>
+    match Eq_eq_dec cod dom with
+    | left edom =>
+      Some (rew [fun x => objs x ~{ C }~> objs cod] edom in @id _ (objs cod))
+    | right _ => None
+    end
+  | cons f nil =>
+    match arrs (snd (get_arrow f)) with
+    | Some (x'; (y'; f)) =>
+      match Eq_eq_dec x' dom, Eq_eq_dec y' cod with
+      | left edom, left ecod =>
+        Some (rew [fun x => objs x  ~{ C }~> objs cod] edom in
+              rew [fun y => objs x' ~{ C }~> objs y] ecod in f)
+      | _, _ => None
+      end
+    | _ => None
+    end
+  | cons f fs =>
+    let '(x, a) := get_arrow f in
+    match arrowsD dom x fs with
+    | Some g =>
+      match arrs a with
+      | Some (x'; (y'; f)) =>
+        match Eq_eq_dec x' x, Eq_eq_dec y' cod with
+        | left edom, left ecod =>
+          Some (rew [fun x => objs x  ~{ C }~> objs cod] edom in
+                rew [fun y => objs x' ~{ C }~> objs y] ecod in f ∘ g)
+        | _, _ => None
+        end
+      | _ => None
+      end
+    | _ => None
+    end
+  end.
+
+(*
+Lemma arrowsD_app x y m f1 f2 f g :
+  arrowsD m y (arrows f1) = Some f ->
+  arrowsD x m (arrows f2) = Some g ->
+  arrowsD x y (arrows (Compose m f1 f2)) ≈ Some (f ∘ g).
+Proof.
+  intros.
+  generalize dependent f2.
+  generalize dependent f.
+  generalize dependent g.
+  generalize dependent m.
+  generalize dependent y.
+  generalize dependent x.
+  induction f1; simpl; intros; equalities.
+  - inversion_clear H.
+    admit.
+  - destruct (arrs _); [|discriminate].
+    destruct s, s; repeat equalities.
+Admitted.
+
+Lemma arrowsD_termD_some x y f r :
+  arrowsD x y (arrows f) = Some r -> termD x y f ≈ Some r.
+Proof.
+  generalize dependent r.
+  generalize dependent y.
+  generalize dependent x.
+  induction f; simpl; intros; repeat equalities; simpl_eq.
+  - inversion_clear H; cat.
+  - destruct (arrs _); [|discriminate].
+    destruct s, s; equalities.
+    equalities'; auto.
+    equalities'; auto.
+    equalities; [|discriminate].
+    inversion_clear H.
+    reflexivity.
+  - rewrite arrowsD_app in H.
+    equalities.
+    specialize (IHf1 _ _ _ a).
+    specialize (IHf2 _ _ _ a0).
+    destruct (termD m y f1) eqn:?, (termD x m f2) eqn:?; try tauto.
+    red in IHf1.
+    red in IHf2.
+    rewrite IHf1, IHf2, b0.
+    reflexivity.
+Qed.
+
+Lemma termD_arrowsD_some x y f r :
+  termD x y f = Some r -> arrowsD x y (arrows f) ≈ Some r.
+Proof.
+  generalize dependent r.
+  generalize dependent y.
+  generalize dependent x.
+  induction f; simpl; intros; repeat equalities; simpl_eq.
+  - inversion_clear H; cat.
+  - destruct (arrs _); [|discriminate].
+    destruct s, s; equalities.
+    equalities'; auto.
+    equalities'; auto.
+    equalities; [|discriminate].
+    inversion_clear H.
+    reflexivity.
+  - destruct (termD m y f1) eqn:?, (termD x m f2) eqn:?; try discriminate.
+    specialize (IHf1 _ _ _ Heqo).
+    specialize (IHf2 _ _ _ Heqo0).
+    inversion_clear H.
+    red in IHf1.
+    red in IHf2.
+    destruct (arrowsD m y (arrows f1)) eqn:?; [|contradiction].
+    destruct (arrowsD x m (arrows f2)) eqn:?; [|contradiction].
+    destruct (arrowsD x y (map (Left m f1 f2) (arrows f1) ++
+                           map (Right m f1 f2) (arrows f2))) eqn:?.
+      apply arrowsD_app in Heqo3.
+      equalities.
+      rewrite <- IHf1, <- IHf2, b0.
+      rewrite a in Heqo1.
+      rewrite a0 in Heqo2.
+      inversion_clear Heqo1.
+      inversion_clear Heqo2.
+      reflexivity.
+    admit.
+Admitted.
+
+Lemma termD_arrowsD_none x y f :
+  termD x y f = None ↔ arrowsD x y (arrows f) = None.
+Proof.
+  generalize dependent y.
+  generalize dependent x.
+  induction f.
+  - destruct (arrs _); auto.
+  - destruct (arrs _); auto.
+  - destruct (termD m y f1) eqn:?.
+      destruct (termD x m f2) eqn:?.
+        discriminate.
+  admit.
+Admitted.
+*)
+
+Fixpoint exprD (e : Expr) : Type :=
   match e with
   | Top           => True
   | Bottom        => False
-  | Equiv x y f g => term_denote x y f ≈ term_denote x y g
-  (* | Not p         => expr_denote p -> False *)
-  | And p q       => expr_denote p ∧ expr_denote q
-  | Or p q        => expr_denote p + expr_denote q
-  | Impl p q      => expr_denote p -> expr_denote q
+  | Equiv x y f g => termD x y f ≈ termD x y g
+  (* | Not p         => exprD p -> False *)
+  | And p q       => exprD p ∧ exprD q
+  | Or p q        => exprD p + exprD q
+  | Impl p q      => exprD p -> exprD q
   end.
+
+Fixpoint exprAD (e : Expr) : Type :=
+  match e with
+  | Top           => True
+  | Bottom        => False
+  | Equiv x y f g => arrowsD x y (arrows f) ≈ arrowsD x y (arrows g)
+  (* | Not p         => exprD p -> False *)
+  | And p q       => exprD p ∧ exprD q
+  | Or p q        => exprD p + exprD q
+  | Impl p q      => exprD p -> exprD q
+  end.
+
+Theorem arrowsD_sound {p dom cod f} :
+  arrowsD dom cod (arrows p) = Some f ->
+  ∃ f', f ≈ f' ∧ termD dom cod p = Some f'.
+Proof.
+Admitted.
+
+Lemma arrowsD_apply dom cod (f g : Term) :
+  arrows_bequiv (arrows f) (arrows g) = true ->
+  arrowsD dom cod (arrows f) ||| false = true ->
+  arrowsD dom cod (arrows f) = arrowsD dom cod (arrows g) ->
+  termD dom cod f ≈ termD dom cod g.
+Proof.
+  intros.
+  destruct (arrowsD dom cod (arrows f)) eqn:?; [|discriminate].
+  destruct (arrowsD_sound Heqo), p.
+  rewrite e0; clear e0.
+  rewrite H1 in Heqo; clear H1.
+  destruct (arrowsD_sound Heqo), p.
+  rewrite e1; clear e1.
+  red.
+  rewrite <- e, <- e0.
+  reflexivity.
+
+  induction f; simpl in *; repeat equalities.
+  - destruct g; simpl in *; repeat equalities.
+    + destruct (arrs a); [|contradiction].
+      destruct s, s; equalities; contradiction.
+    + destruct (arrowsD x x (map (Left m g1 g2) (arrows g1) ++
+                             map (Right m g1 g2) (arrows g2))) eqn:?;
+      [|contradiction].
+      admit.
+  - destruct g; simpl in *; repeat equalities.
+    + destruct (arrs a); auto.
+    + destruct (arrowsD _ _ _) eqn:?; [contradiction|].
+        admit.
+  - admit.
+Admitted.
+
+Lemma exprAD_sound (e : Expr) : exprAD e -> exprD e.
+Proof.
+  destruct e; auto; intros.
+  red in X; red.
+  apply arrowsD_sound; auto.
+Qed.
 
 End Denote.
 
@@ -73,7 +265,7 @@ Variables f g h : x ~> x.
 
 Definition objs := (fun _ : obj_idx => x).
 
-Eval simpl in @expr_denote C objs
+Eval simpl in @exprD C objs
   (fun i => if Pos.eqb i 1 then Some (1; (1; f)) else
             if Pos.eqb i 2 then Some (1; (1; g)) else Some (1; (1; h)))%positive
   (Equiv 1 1 (@Compose 1 (@Morph 1) (@Compose 1 (@Morph 2) (@Morph 3)))
