src/Normal.v
@@ -22,6 +22,110 @@ Section Normal.
 
 Import EqNotations.
 
+Inductive Arrow : Term -> Set :=
+  | Here  : ∀ x y a, Arrow (Morph x y a)
+  | Left  : ∀ (m : obj_idx) f g, Arrow f -> Arrow (Compose m f g)
+  | Right : ∀ (m : obj_idx) f g, Arrow g -> Arrow (Compose m f g).
+
+Definition Arrow_inv_t : forall t, Arrow t -> Type.
+Proof.
+  intros [] H.
+  - exact False.
+  - exact (H = Here x y a).
+  - exact ((∃ H', H = Left m f g H') + (∃ H', H = Right m f g H')).
+Defined.
+
+Lemma Arrow_inv t f : Arrow_inv_t t f.
+Proof.
+  destruct f; simpl; equalities; simpl_eq; auto.
+  - left. exists f0; auto.
+  - right. exists f0; auto.
+Defined.
+
+Lemma Arrow_Morph `(H : Arrow (Morph x y a)) : H = Here x y a.
+Proof. exact (Arrow_inv _ H). Defined.
+
+Lemma Arrow_Compose `(H : Arrow (Compose m f g)) :
+  (∃ H', H = Left m f g H') + (∃ H', H = Right m f g H').
+Proof. exact (Arrow_inv _ H). Defined.
+
+Fixpoint get_arrow `(f : Arrow t) : obj_idx * arr_idx :=
+  match f with
+  | Here x _ a    => (x, a)
+  | Left _ _ _ x  => get_arrow x
+  | Right _ _ _ x => get_arrow x
+  end.
+
+Function arrow_bequiv {t t' : Term} (p : Arrow t) (q : Arrow t') : bool :=
+  match get_arrow p, get_arrow q with
+  | (o, f), (o', f') => Eq_eqb o o' && Eq_eqb f f'
+  end.
+
+Lemma arrow_bequiv_eq {t t' : Term} (p : Arrow t) (q : Arrow t') :
+  arrow_bequiv p q = true -> get_arrow p = get_arrow q.
+Proof.
+Admitted.
+(*
+  destruct (term_beq t t') eqn:?.
+  - apply term_beq_eq in Heqb; subst; intros.
+    exists eq_refl; simpl.
+    generalize dependent q.
+    induction p; simpl; intros; equalities.
+    + pose proof (Arrow_Morph q); auto.
+    + destruct (Arrow_Compose q), s; subst.
+        now rewrite (IHp _ H1).
+      discriminate.
+    + destruct (Arrow_Compose q), s; subst.
+        discriminate.
+      now rewrite (IHp _ H1).
+  - intros.
+    rewrite arrow_beq_equation, Heqb in H.
+    discriminate.
+Qed.
+*)
+
+Function arrows (t : Term) : list (Arrow t) :=
+  match t with
+  | Identity _    => nil
+  | Morph x y a   => [Here x y a]
+  | Compose m f g => map (Left m f g) (arrows f) ++
+                     map (Right m f g) (arrows g)
+  end.
+
+Function arrows_bequiv {t t' : Term}
+         (ps : list (Arrow t)) (qs : list (Arrow t')) : bool :=
+  term_beq t t' &&&
+  match ps, qs with
+  | nil, nil => true
+  | cons p ps, cons q qs =>
+    arrow_bequiv p q &&& arrows_bequiv ps qs
+  | _, _ => false
+  end.
+
+(*
+Fixpoint arrows_bequiv_eq {t t' : Term}
+         (ps : list (Arrow t)) (qs : list (Arrow t')) :
+  arrows_beq ps qs = true
+    -> { H : t' = t | ps = rew [fun t => list (Arrow t)] H in qs }.
+Proof.
+  intros.
+  rewrite arrows_beq_equation in H.
+  destruct (term_beq t t') eqn:?; [|discriminate].
+  apply term_beq_eq in Heqb; subst.
+  exists eq_refl; simpl.
+  induction ps, qs; auto; try discriminate.
+  equalities.
+  apply arrow_beq_eq in H0.
+  destruct H0; subst; simpl; simpl_eq.
+  apply arrows_beq_eq in H1.
+  destruct H1.
+  rewrite e.
+  f_equal; clear.
+  destruct t'.
+  inversion a0.
+Qed.
+*)
+
 (* Notation Term    := (Term arrs). *)
 (* Notation TermDom := (TermDom arrs). *)
 (* Notation TermCod := (TermCod arrs). *)
