src/Decide.v
@@ -15,6 +15,7 @@ Require Import Category.Theory.Functor.
 Require Import Solver.Lib.
 Require Import Solver.Expr.
 Require Import Solver.Denote.
+Require Import Solver.Normal.
 
 Generalizable All Variables.
 
@@ -22,7 +23,7 @@ Section Decide.
 
 Program Definition Term_Category {C objs arrs} : Category := {|
   obj := obj_idx;
-  hom := fun x y => ∃ f f', @term_denote C objs arrs x y f = Some f';
+  hom := fun x y => ∃ f f', @termD C objs arrs x y f = Some f';
   homset := fun x y => {| equiv := fun f g => `1 `2 f ≈ `1 `2 g |};
   id := fun x => (Identity x; (@id C (objs x); _));
   compose := fun x y z f g => (Compose y `1 f `1 g; (`1 `2 f ∘ `1 `2 g; _))
@@ -34,55 +35,55 @@ Program Definition Term_Category' {C objs arrs} : Category := {|
   obj := obj_idx;
   hom := fun _ _ => Term;
   homset := fun x y => {| equiv := fun f g =>
-    @term_denote C objs arrs x y f ≈ @term_denote C objs arrs x y g |};
+    @termD C objs arrs x y f ≈ @termD C objs arrs x y g |};
   id := Identity;
   compose := fun _ y _ => Compose y
 |}.
 Next Obligation.
   equivalence.
-  - destruct (term_denote objs arrs x y x0) eqn:?; auto.
+  - destruct (termD objs arrs x y x0) eqn:?; auto.
     reflexivity.
-  - destruct (term_denote objs arrs x y x0) eqn:?;
-    destruct (term_denote objs arrs x y y0) eqn:?; auto.
+  - destruct (termD objs arrs x y x0) eqn:?;
+    destruct (termD objs arrs x y y0) eqn:?; auto.
     now symmetry.
-  - destruct (term_denote objs arrs x y x0) eqn:?;
-    destruct (term_denote objs arrs x y y0) eqn:?;
-    destruct (term_denote objs arrs x y z) eqn:?; auto.
+  - destruct (termD objs arrs x y x0) eqn:?;
+    destruct (termD objs arrs x y y0) eqn:?;
+    destruct (termD objs arrs x y z) eqn:?; auto.
       now transitivity h0.
     contradiction.
 Defined.
 Next Obligation.
   proper.
-  destruct (term_denote objs arrs y z x0) eqn:?;
-  destruct (term_denote objs arrs x y x1) eqn:?;
-  destruct (term_denote objs arrs y z y0) eqn:?;
-  destruct (term_denote objs arrs x y y1) eqn:?; auto.
+  destruct (termD objs arrs y z x0) eqn:?;
+  destruct (termD objs arrs x y x1) eqn:?;
+  destruct (termD objs arrs y z y0) eqn:?;
+  destruct (termD objs arrs x y y1) eqn:?; auto.
   now rewrite X, X0.
 Defined.
 Next Obligation.
   equalities'; auto.
   equalities.
-  destruct (term_denote objs arrs x y f) eqn:?; cat.
+  destruct (termD objs arrs x y f) eqn:?; cat.
 Qed.
 Next Obligation.
   equalities'; auto.
   equalities.
-  destruct (term_denote objs arrs x y f) eqn:?; cat.
+  destruct (termD objs arrs x y f) eqn:?; cat.
 Qed.
 Next Obligation.
-  destruct (term_denote objs arrs z w f) eqn:?;
-  destruct (term_denote objs arrs y z g) eqn:?;
-  destruct (term_denote objs arrs x y h) eqn:?; cat.
+  destruct (termD objs arrs z w f) eqn:?;
+  destruct (termD objs arrs y z g) eqn:?;
+  destruct (termD objs arrs x y h) eqn:?; cat.
 Qed.
 Next Obligation.
-  destruct (term_denote objs arrs z w f) eqn:?;
-  destruct (term_denote objs arrs y z g) eqn:?;
-  destruct (term_denote objs arrs x y h) eqn:?; cat.
+  destruct (termD objs arrs z w f) eqn:?;
+  destruct (termD objs arrs y z g) eqn:?;
+  destruct (termD objs arrs x y h) eqn:?; cat.
 Qed.
 
 Existing Instance Term_Category'.
 
-Lemma term_denote_append C objs arrs x y (f1 : Term) :
+Lemma termD_append C objs arrs x y (f1 : Term) :
   (f1 : @hom (@Term_Category' C objs arrs) x y) ≈ term_normal f1.
 Proof.
   simpl.
@@ -96,8 +97,8 @@ Proof.
     equalities'; auto.
     equalities; reflexivity.
   - specialize (IHf1_1 m y).
-    destruct (term_denote objs arrs m y f1_1) eqn:?;
-    destruct (term_denote objs arrs m y (term_append f1_1 (Identity m))) eqn:?.
+    destruct (termD objs arrs m y f1_1) eqn:?;
+    destruct (termD objs arrs m y (term_append f1_1 (Identity m))) eqn:?.
 Admitted.
 
 Program Definition term_rect' x y (f : Term) :
@@ -118,37 +119,34 @@ Next Obligation. Admitted.
 Next Obligation. Admitted.
 
 Lemma term_normal_compose C objs arrs x m y f1 f2 f' g' :
-  term_denote objs arrs m y (term_normal f1) ≈ Some f' ->
-  term_denote objs arrs x m (term_normal f2) ≈ Some g' ->
-  @term_denote C objs arrs x y (term_normal (Compose m f1 f2)) ≈
-  @term_denote C objs arrs x y (Compose m (term_normal f1) (term_normal f2)).
+  termD objs arrs m y (term_normal f1) ≈ Some f' ->
+  termD objs arrs x m (term_normal f2) ≈ Some g' ->
+  @termD C objs arrs x y (term_normal (Compose m f1 f2)) ≈
+  @termD C objs arrs x y (Compose m (term_normal f1) (term_normal f2)).
 Proof.
   intros.
   unfold term_normal in *.
   simpl term_append in *.
-  rewrite X0.
-  destruct (term_denote objs arrs m y (term_normal f1)) eqn:?; [|contradiction].
-  destruct (term_denote objs arrs x m (term_normal f2)) eqn:?; [|contradiction].
 Admitted.
 
-Lemma term_denote_term_append C objs arrs x m y f1 f2 f' g' :
-  term_denote objs arrs m y (term_normal f1) ≈ Some f' ->
-  term_denote objs arrs x m (term_normal f2) ≈ Some g' ->
-  @term_denote C objs arrs x y (term_normal (Compose m f1 f2)) ≈ Some (f' ∘ g').
+Lemma termD_term_append C objs arrs x m y f1 f2 f' g' :
+  termD objs arrs m y (term_normal f1) ≈ Some f' ->
+  termD objs arrs x m (term_normal f2) ≈ Some g' ->
+  @termD C objs arrs x y (term_normal (Compose m f1 f2)) ≈ Some (f' ∘ g').
 Proof.
   intros.
   rewrite term_normal_compose; eauto.
   simpl.
-  destruct (term_denote objs arrs m y (term_normal f1)); auto.
-  destruct (term_denote objs arrs x m (term_normal f2)); auto.
+  destruct (termD objs arrs m y (term_normal f1)); auto.
+  destruct (termD objs arrs x m (term_normal f2)); auto.
   red in X.
   red in X0.
   cat.
 Qed.
 
 Lemma normalize_equiv C objs arrs x y f f' :
-  @term_denote C objs arrs x y f = Some f' ->
-  @term_denote C objs arrs x y (term_normal f) ≈ Some f'.
+  @termD C objs arrs x y f = Some f' ->
+  @termD C objs arrs x y (term_normal f) ≈ Some f'.
 Proof.
   intros.
   generalize dependent y.
@@ -166,17 +164,17 @@ Proof.
     inversion_clear H.
     reflexivity.
   - simpl in H.
-    destruct (term_denote _ _ _ _ f1) eqn:?; [|discriminate].
-    destruct (term_denote _ _ _ _ f2) eqn:?; [|discriminate].
+    destruct (termD _ _ _ _ f1) eqn:?; [|discriminate].
+    destruct (termD _ _ _ _ f2) eqn:?; [|discriminate].
     inversion_clear H.
     specialize (IHf1 _ _ _ Heqo); clear Heqo.
     specialize (IHf2 _ _ _ Heqo0); clear Heqo0.
-    now apply term_denote_term_append.
+    now apply termD_term_append.
 Qed.
 
 Lemma normalize_decides C objs arrs x y f f' g g' :
-  @term_denote C objs arrs x y f = Some f' ->
-  @term_denote C objs arrs x y g = Some g' ->
+  @termD C objs arrs x y f = Some f' ->
+  @termD C objs arrs x y g = Some g' ->
   term_beq (term_normal f) (term_normal g) = true ->
   f' ≈ g'.
 Proof.
@@ -187,6 +185,66 @@ Proof.
   rewrite <- H1 in H0.
   rewrite H in H0.
   now red in H0.
+Qed.
+
+Lemma arrows_decide C objs arrs x y f f' g g' :
+  @termD C objs arrs x y f = Some f' ->
+  @termD C objs arrs x y g = Some g' ->
+  arrows_bequiv (arrows f) (arrows g) = true ->
+  f' ≈ g'.
+Proof.
+  intros.
+  generalize dependent g'.
+  generalize dependent f'.
+  generalize dependent g.
+  generalize dependent y.
+  generalize dependent x.
+  induction f; simpl; intros; equalities.
+  - destruct g; simpl in *; equalities; simpl_eq.
+    + inversion_clear H.
+      inversion_clear H0.
+      reflexivity.
+    + destruct (arrs _); [|discriminate].
+      destruct s, s; equalities.
+    + discriminate.
+  - destruct g; simpl in *; equalities; simpl_eq.
+    + destruct (arrs _); [|discriminate].
+      destruct s, s; equalities.
+      inversion H; subst.
+      inversion H0; subst.
+      reflexivity.
+    + destruct (arrs _); [|discriminate].
+      destruct s, s; equalities.
+  - destruct g; simpl in *; equalities; simpl_eq;
+    (destruct (termD _ _ _ _ f1) eqn:?; [|discriminate]);
+    (destruct (termD _ _ _ _ f2) eqn:?; [|discriminate]).
+    + inversion H; subst; clear H.
+      inversion H0; subst; clear H0.
+      clear -H1 Heqo0 Heqo1.
+      destruct (arrows f1) eqn:?; simpl in H1; [|discriminate].
+      destruct (arrows f2) eqn:?; simpl in H1; discriminate.
+    + destruct (arrs _); [|discriminate].
+      destruct s, s; equalities.
+      inversion H; subst; clear H.
+      inversion H0; subst; clear H0.
+      destruct (arrows f1) eqn:?; simpl in H1; [|discriminate].
+      destruct (arrows f2) eqn:?; simpl in H1; discriminate.
+    + destruct (termD _ _ _ _ g1) eqn:?; [|discriminate].
+      destruct (termD _ _ _ _ g2) eqn:?; [|discriminate].
+      inversion H; subst; clear H.
+      inversion H0; subst; clear H0.
+      destruct (arrows f1) eqn:?; simpl in H1;
+      destruct (arrows f2) eqn:?; simpl in H1;
+      destruct (arrows g1) eqn:?; simpl in H1;
+      destruct (arrows g2) eqn:?; simpl in H1;
+      equalities; try discriminate;
+      repeat match goal with
+      | [ H : term_beq _ _ = true |- _ ] => 
+        apply term_beq_eq in H; subst
+      end;
+      rewrite Heqo in Heqo1; inversion_clear Heqo1;
+      rewrite Heqo0 in Heqo2; inversion_clear Heqo2;
+      reflexivity.
 Qed.
 
 End Decide.
